Use iris.bi.interface instead of our own

theories/Sep/Logic.v
@@ -26,585 +26,84 @@
 (* SOFTWARE, EVEN IF ADVISED OF THE POSSIBILITY OF SUCH DAMAGE.               *)
 (******************************************************************************)
 
-From Coq Require Import
-     Classes.Morphisms
-     Classes.RelationClasses
-     Program.Basics
-     Setoid.
+From iris.bi Require Export interface derived_laws.
+From Katamaran Require Import Context Environment Prelude.
 
-From Katamaran Require Import
-     Context
-     Environment
-     Notations.
+Section WithBi.
+  Context {L : bi}.
 
-Local Set Implicit Arguments.
+  Lemma forall_elim' {A : Type} (a : A) (Ψ : A → L) Φ :
+    (Ψ a ⊢ Φ) → (bi_forall Ψ ⊢ Φ).
+  Proof. intros. transitivity (Ψ a); auto. apply bi.forall_elim. Qed.
 
-Declare Scope logic_scope.
-Delimit Scope logic_scope with logic.
-Delimit Scope logic_scope with L.
+  Section Forall.
 
-Module sep.
-
-  Structure SepLogic :=
-    { lcar        :> Type;
-      lentails    : lcar -> lcar -> Prop where "P ⊢ Q" := (lentails P Q);
-      land        : lcar -> lcar -> lcar where "P ∧ Q" := (land P Q);
-      lor         : lcar -> lcar -> lcar where "P ∨ Q" := (lor P Q);
-      limpl       : lcar -> lcar -> lcar where "P → Q" := (limpl P Q);
-      lprop       : Prop -> lcar where "'!!' P" := (lprop P);
-      lex         : forall T, (T -> lcar) -> lcar;
-      lall        : forall T, (T -> lcar) -> lcar;
-      lemp        : lcar;
-      lsep        : lcar -> lcar -> lcar where "P ∗ Q" := (lsep P Q);
-      lwand       : lcar -> lcar -> lcar where "P -∗ Q" := (lwand P Q);
-
-      lequiv (P Q : lcar) : Prop := (P ⊢ Q) /\ (Q ⊢ P) where "P ⊣⊢ Q" := (lequiv P Q);
-
-      #[canonical=no] lentails_preorder  : PreOrder lentails;
-
-      #[canonical=no] land_right X P Q         : (X ⊢ P) -> (X ⊢ Q) -> (X ⊢ P ∧ Q);
-      #[canonical=no] land_left1 P Q R         : (P ⊢ R) -> (P ∧ Q ⊢ R);
-      #[canonical=no] land_left2 P Q R         : (Q ⊢ R) -> (P ∧ Q ⊢ R);
-      #[canonical=no] lor_left P Q R           : (P ⊢ R) -> (Q ⊢ R) -> (P ∨ Q ⊢ R);
-      #[canonical=no] lor_right1 P Q R         : (P ⊢ Q) -> (P ⊢ Q ∨ R);
-      #[canonical=no] lor_right2 P Q R         : (P ⊢ R) -> (P ⊢ Q ∨ R);
-      #[canonical=no] lex_right B x P Q        : (P ⊢ Q x) -> (P ⊢ @lex B Q);
-      #[canonical=no] lex_left B P Q           : (forall x, P x ⊢ Q) -> (@lex B P ⊢ Q);
-      #[canonical=no] lall_left B x P Q        : (P x ⊢ Q) -> (@lall B P ⊢ Q);
-      #[canonical=no] lall_right B P Q         : (forall v, P ⊢ Q v) -> (P ⊢ @lall B Q);
-      #[canonical=no] limpl_and_adjoint P Q R  : (P ∧ Q ⊢ R) <-> (P ⊢ Q → R);
-      #[canonical=no] lprop_left (P : Prop) Q  : (P -> (!!True ⊢ Q)) -> (!!P ⊢ Q);
-      #[canonical=no] lprop_right (P : Prop) Q : P -> (Q ⊢ !!P);
-
-      #[canonical=no] lsep_assoc P Q R        : P ∗ (Q ∗ R) ⊣⊢ (P ∗ Q) ∗ R;
-      #[canonical=no] lsep_comm P Q           : P ∗ Q ⊣⊢ Q ∗ P;
-      #[canonical=no] lwand_sep_adjoint P Q R : (P ∗ Q ⊢ R) <-> (P ⊢ Q -∗ R);
-      #[canonical=no] lsep_andp_prop P Q R    : P ∗ (!!Q ∧ R) ⊣⊢ !!Q ∧ (P ∗ R);
-      #[canonical=no] lsep_entails P P' Q Q'  : (P ⊢ P') -> (Q ⊢ Q') -> (P ∗ Q ⊢ P' ∗ Q');
-      #[canonical=no] lsep_emp P              : P ∗ lemp ⊣⊢ P;
-      #[canonical=no] lsep_leak P             : P ⊢ lemp;
-    }.
-
-  #[global] Arguments lequiv {_} _ _.
-  #[global] Arguments lentails {_} _ _.
-  #[global] Arguments land {_} _ _.
-  #[global] Arguments lor {_} _ _.
-  #[global] Arguments limpl {_} _ _.
-  #[global] Arguments lprop {_} _.
-  #[global] Arguments lex {_} [_] _.
-  #[global] Arguments lall {_} [_] _.
-  #[global] Arguments lemp {_}.
-  #[global] Arguments lsep {_} _ _.
-  #[global] Arguments lwand {_} _ _.
-
-  #[global] Arguments lex_right {_} [_] _.
-  #[global] Arguments lall_left {_} [_] _.
-
-  Module Import notations.
-    Open Scope logic_scope.
-    Notation "P ⊢ Q" := (lentails P%L Q%L) : type_scope.
-    Notation "P '⊢@{' L } Q" := (@lentails L P%L Q%L) (only parsing) : type_scope.
-    Notation "P ⊣⊢ Q" := (lequiv P%L Q%L) : type_scope.
-    Notation "P '⊣⊢@{' L } Q" := (@lequiv L P%L Q%L) (only parsing) : type_scope.
-
-    Infix "∨" := lor : logic_scope.
-    Infix "∧" := land : logic_scope.
-    Infix "→" := limpl : logic_scope.
-    Notation "'∃' x .. y , P " :=
-      (lex (fun x => .. (lex (fun y => P)) ..))
-      (at level 200, x binder, y binder, right associativity,
-      format "'[  ' '[  ' ∃  x  ..  y ']' ,  '/' P ']'") : logic_scope.
-    Notation "'∀' x .. y , P " :=
-      (lall (fun x => .. (lall (fun y => P)) ..))
-      (at level 200, x binder, y binder, right associativity,
-      format "'[  ' '[  ' ∀  x  ..  y ']' ,  '/' P ']'") : logic_scope.
-    Notation "'!!' e" := (lprop e) : logic_scope.
-    Notation "⊤" := (lprop True) : logic_scope.
-    Notation "⊥" := (lprop False) : logic_scope.
-    Infix "∗" := lsep : logic_scope.
-    Infix "-∗" := lwand : logic_scope.
-  End notations.
-
-  Module Import instances.
-
-    #[export] Existing Instance lentails_preorder.
-    #[export] Instance lentails_rewrite_relation {L} :
-      RewriteRelation (@lentails L) := {}.
-
-    #[export] Instance lequiv_equivalence {L} : Equivalence (@lequiv L).
-    Proof.
-      constructor.
-      - intros P. split; reflexivity.
-      - intros P Q [pq qp]; split; assumption.
-      - intros P Q R [pq qp] [qr rq].
-        split; transitivity Q; auto.
-    Qed.
-
-    #[export] Instance lequiv_entails_subrelation {L} :
-      subrelation (@lequiv L) (@lentails L).
-    Proof. firstorder. Qed.
-
-    #[export] Instance lequiv_flip_entails_subrelation {L} :
-      subrelation (@lequiv L) (flip (@lentails L)).
-    Proof. firstorder. Qed.
-
-    #[export] Instance proper_entails_equiv_iff {L} :
-      Proper (lequiv ==> lequiv ==> iff) (@lentails L).
-    Proof. intros P Q pq R S rs. split; now rewrite pq, rs. Qed.
-
-    #[export] Instance proper_entails_entails_impl {L} :
-      Proper (lentails --> lentails ==> impl) (@lentails L).
-    Proof.
-      unfold Proper, respectful, flip, impl.
-      intros P Q qp R S rs pr.
-      transitivity P; auto.
-      transitivity R; auto.
-    Qed.
-
-    #[export] Instance proper_land_entails {L} :
-      Proper (lentails ==> lentails ==> lentails) (@land L).
-    Proof. intros P Q pq R S rs. apply land_right; [apply land_left1 | apply land_left2]; assumption. Qed.
-
-    #[export] Instance proper_land_equiv {L} :
-      Proper (lequiv ==> lequiv ==> lequiv) (@land L).
-    Proof. intros P Q [pq qp] R S [rs sr]. split; now apply proper_land_entails. Qed.
-
-    #[export] Instance proper_lor_entails {L} : Proper (lentails ==> lentails ==> lentails) (@lor L).
-    Proof. intros P Q pq R S rs. apply lor_left; [ apply lor_right1 | apply lor_right2]; assumption. Qed.
-
-    #[export] Instance proper_lor_equiv {L} : Proper (lequiv ==> lequiv ==> lequiv) (@lor L).
-    Proof. intros P Q [pq qp] R S [rs sr]. split; now apply proper_lor_entails. Qed.
-
-    #[export] Instance proper_limpl_entails {L} : Proper (lentails --> lentails ==> lentails) (@limpl L).
-    Proof.
-      intros P Q pq R S rs.
-      apply limpl_and_adjoint.
-      rewrite <- pq, <- rs.
-      apply limpl_and_adjoint.
-      reflexivity.
-    Qed.
-
-    #[export] Instance proper_limpl_equiv {L} : Proper (lequiv ==> lequiv ==> lequiv) (@limpl L).
-    Proof. intros P Q [pq] R S [rs]. split; apply proper_limpl_entails; auto. Qed.
-
-    #[export] Instance proper_lprop_entails {L} : Proper (impl ==> lentails) (@lprop L).
-    Proof. intros P Q pq. apply lprop_left; intro; now apply lprop_right, pq. Qed.
-
-    #[export] Instance proper_lprop_equiv {L} : Proper (iff ==> lequiv) (@lprop L).
-    Proof. intros P Q pq. split; apply proper_lprop_entails; unfold impl; apply pq. Qed.
-
-    #[export] Instance proper_lex_entails {L} T : Proper (pointwise_relation T lentails ==> lentails) (@lex L T).
-    Proof. intros P Q pq. apply lex_left; intro x; apply (lex_right x), (pq x). Qed.
-
-    #[export] Instance proper_lex_equiv {L} T : Proper (pointwise_relation T lequiv ==> lequiv) (@lex L T).
-    Proof. intros P Q pq. split; apply lex_left; intro x; apply (lex_right x), (pq x). Qed.
-
-    #[export] Instance proper_lall_entails {L} T : Proper (pointwise_relation T lentails ==> lentails) (@lall L T).
-    Proof. intros P Q pq. apply lall_right; intro x; apply (lall_left x), (pq x). Qed.
-
-    #[export] Instance proper_lall_equiv {L} T : Proper (pointwise_relation T lequiv ==> lequiv) (@lall L T).
-    Proof. intros P Q pq. split; apply lall_right; intro x; apply (lall_left x), (pq x). Qed.
-
-    #[export] Instance proper_lsep_entails {L} : Proper (lentails ==> lentails ==> lentails) (@lsep L).
-    Proof. intros P Q pq R S rs. now apply lsep_entails. Qed.
-
-    #[export] Instance proper_lsep_equiv {L} : Proper (lequiv ==> lequiv ==> lequiv) (@lsep L).
-    Proof. intros P Q [pq qp] R S [rs sr]. split; now apply lsep_entails. Qed.
-
-    #[export] Instance proper_lwand_entails {L} : Proper (lentails --> lentails ==> lentails) (@lwand L).
-    Proof.
-      intros P Q pq R S rs.
-      apply lwand_sep_adjoint.
-      rewrite <- pq, <- rs.
-      now apply lwand_sep_adjoint.
-    Qed.
-
-    #[export] Instance proper_lwand_equiv {L} : Proper (lequiv ==> lequiv ==> lequiv) (@lwand L).
-    Proof. intros P Q [pq qp] R S [rs sr]. split; now apply proper_lwand_entails. Qed.
-
-  End instances.
-
-  Section Derived.
-
-    Context {L : SepLogic} (B : Set) (D : B -> Set).
+    Context {B : Set} {D : B -> Set}.
 
     Fixpoint Forall {Δ : Ctx B} : (Env D Δ -> L) -> L :=
       match Δ with
       | ctx.nil      => fun P => P env.nil
-      | ctx.snoc Δ b => fun P => Forall (fun E => lall (fun v => P (env.snoc E b v)))
-      end.
+      | ctx.snoc Δ b => fun P => Forall (fun E => ∀ v, P (env.snoc E b v))
+      end%I.
 
     Lemma Forall_forall (Δ : Ctx B) (P : Env D Δ -> L) :
       (Forall P) ⊣⊢ (∀ E : Env D Δ, P E).
     Proof.
       induction Δ; cbn.
-      - split.
-        + apply lall_right. intros E. env.destroy E. reflexivity.
-        + apply (lall_left env.nil). reflexivity.
+      - apply bi.entails_anti_sym.
+        + apply bi.forall_intro; intros E. now env.destroy E.
+        + apply bi.forall_elim.
       - rewrite IHΔ. clear IHΔ.
-        split; apply lall_right.
+        apply bi.entails_anti_sym; apply bi.forall_intro.
         + intros E. destruct (env.view E) as [E v].
-          now apply (lall_left E), (lall_left v).
-        + intros E. apply lall_right. intros v.
-          now apply (lall_left (env.snoc E _ v)).
+          now apply (forall_elim' E), (forall_elim' v).
+        + intros E. apply bi.forall_intro. intros v.
+          now apply (forall_elim' (env.snoc E _ v)).
     Qed.
 
-  End Derived.
+  End Forall.
 
-  Section Facts.
+  Lemma wand_or_distr {P Q R : L} :
+    ((P ∨ Q) -∗ R) ⊣⊢ ((P -∗ R) ∧ (Q -∗ R)).
+  Proof.
+    apply bi.entails_anti_sym.
+    - apply bi.and_intro; apply bi.wand_mono; try easy.
+      apply bi.or_intro_l. apply bi.or_intro_r.
+    - apply bi.wand_intro_r.
+      rewrite bi.sep_comm.
+      apply bi.wand_elim_l'.
+      apply bi.or_elim.
+      + apply bi.wand_intro_r.
+        rewrite bi.and_elim_l.
+        apply bi.wand_elim_r.
+      + apply bi.wand_intro_r.
+        rewrite bi.and_elim_r.
+        apply bi.wand_elim_r.
+  Qed.
 
-    Context {L : SepLogic}.
+  Lemma wand_sep_adjoint {P Q R : L} :
+    (P ∗ Q ⊢ R) <-> (P ⊢ Q -∗ R).
+  Proof. split. apply bi.wand_intro_r. apply bi.wand_elim_l'. Qed.
 
-    Lemma ltrue_right {P : L} : P ⊢ ⊤.
-    Proof. now apply lprop_right. Qed.
+  Lemma entails_wand_iff {P Q : L} :
+    (P ⊢ Q) ↔ (P -∗ Q).
+  Proof. split. apply bi.entails_wand. apply bi.wand_entails. Qed.
 
-    Lemma lfalse_left {P : L} : ⊥ ⊢ P.
-    Proof. now apply lprop_left. Qed.
+  Lemma entails_mono' : Proper (flip (⊢) ==> (⊢) ==> impl) (bi_entails : relation L).
+  Proof.
+    intros P Q QP R S RS. intros H.
+    transitivity P; auto.
+    transitivity R; auto.
+  Qed.
 
-    Lemma land_assoc {P Q R : L} :
-      (P ∧ Q) ∧ R ⊣⊢ P ∧ (Q ∧ R).
-    Proof.
-      split; repeat apply land_right.
-      - now apply land_left1, land_left1.
-      - now apply land_left1, land_left2.
-      - now apply land_left2.
-      - now apply land_left1.
-      - now apply land_left2, land_left1.
-      - now apply land_left2, land_left2.
-    Qed.
+  Lemma entails_apply {P Q : L} :
+    (True ⊢ P) -> ((P → Q) ⊢ Q).
+  Proof.
+    intros H. transitivity ((P → Q) ∧ P)%I.
+    - apply bi.and_intro. easy.
+      transitivity (@bi_pure L True); auto.
+      apply bi.True_intro.
+    - apply bi.impl_elim_l.
+  Qed.
 
-    Lemma land_false {P : L} : P ∧ ⊥ ⊣⊢ ⊥.
-    Proof.
-      split.
-      - apply land_left2, lfalse_left.
-      - apply lfalse_left.
-    Qed.
-
-    Lemma lfalse_and {P : L} : ⊥ ∧ P ⊣⊢ ⊥.
-    Proof.
-      split.
-      - apply land_left1, lfalse_left.
-      - apply lfalse_left.
-    Qed.
-
-    Lemma lex_false {T} : (∃ _ : T, ⊥) ⊣⊢@{L} ⊥.
-    Proof.
-      split.
-      - apply lex_left. intros _. apply lfalse_left.
-      - apply lfalse_left.
-    Qed.
-
-    Lemma land_comm {P Q : L} :
-      P ∧ Q ⊣⊢ Q ∧ P.
-    Proof.
-      split; (apply land_right; [ now apply land_left2 | now apply land_left1 ]).
-    Qed.
-
-    Lemma land_idem {P : L} :
-      P ∧ P ⊣⊢ P.
-    Proof.
-      split.
-      - now apply land_left1.
-      - now apply land_right.
-    Qed.
-
-    Lemma land_true {P : L} :
-      P ∧ ⊤ ⊣⊢ P.
-    Proof.
-      split.
-      - now apply land_left1.
-      - apply land_right.
-        + reflexivity.
-        + apply ltrue_right.
-    Qed.
-
-    Lemma lor_assoc {P Q R : L} :
-      ((P ∨ Q) ∨ R) ⊣⊢ (P ∨ (Q ∨ R)).
-    Proof.
-      split; repeat apply lor_left.
-      - now apply lor_right1.
-      - now apply lor_right2, lor_right1.
-      - now apply lor_right2, lor_right2.
-      - now apply lor_right1, lor_right1.
-      - now apply lor_right1, lor_right2.
-      - now apply lor_right2.
-    Qed.
-
-    Lemma lor_comm {P Q : L} :
-      (P ∨ Q) ⊣⊢ (Q ∨ P).
-    Proof.
-
-      split; (apply lor_left; [ apply lor_right2 | apply lor_right1 ]); reflexivity.
-    Qed.
-
-    Lemma lor_idem {P : L} :
-      (P ∨ P) ⊣⊢ P.
-    Proof.
-      split.
-      - now apply lor_left.
-      - now apply lor_right1.
-    Qed.
-
-    Lemma lprop_and_distr {P Q : Prop} :
-      (!! P) ∧ (!! Q) ⊣⊢@{L} !! (P /\ Q).
-    Proof.
-      split.
-      - apply limpl_and_adjoint.
-        apply lprop_left; intros.
-        apply limpl_and_adjoint.
-        apply land_left2.
-        apply lprop_left; intros.
-        apply lprop_right.
-        split; assumption.
-      - apply lprop_left; intros [].
-        apply land_right; apply lprop_right; assumption.
-    Qed.
-
-    Lemma lprop_float {P : L} {Q : Prop} :
-      (P ∧ !! Q) ⊣⊢ (!! Q ∧ P).
-    Proof. apply land_comm. Qed.
-
-    Lemma lemp_true :
-      lemp ⊣⊢@{L} ⊤.
-    Proof.
-      split.
-      apply ltrue_right.
-      apply lsep_leak.
-    Qed.
-
-    Lemma lsep_true (P : L) : ⊤ ∗ P ⊣⊢ P.
-    Proof.
-      rewrite <- lemp_true.
-      rewrite lsep_comm.
-      rewrite lsep_emp.
-      reflexivity.
-    Qed.
-
-    Lemma lprop_sep_distr Q P :
-      !! P ∗ !! Q ⊣⊢@{L} !! (P /\ Q).
-    Proof.
-      split.
-      - apply lwand_sep_adjoint.
-        apply lprop_left. intros HP.
-        apply lwand_sep_adjoint.
-        rewrite lsep_true.
-        apply lprop_left. intros HQ.
-        apply lprop_right; auto.
-      - apply lprop_left. intros [HP HQ].
-        rewrite <- lsep_true at 1.
-        apply lsep_entails; now apply lprop_right.
-    Qed.
-
-    Lemma lprop_or_distr {P Q : Prop} :
-      (!! P) ∨ (!! Q) ⊣⊢@{L} !! (P \/ Q).
-    Proof.
-      split.
-      - apply lor_left; apply lprop_left;
-          intros H; apply lprop_right; auto.
-      - apply lprop_left; intros [HP|HQ];
-          [apply lor_right1 | apply lor_right2];
-          now apply lprop_right.
-    Qed.
-
-    Lemma lprop_exists_comm {T} (P : T -> Prop) :
-      !! (exists t : T, P t) ⊣⊢@{L} (∃ t : T, !! P t).
-    Proof.
-      split.
-      - apply lprop_left; intros [x HP].
-        apply lex_right with x.
-        now apply lprop_right.
-      - apply lex_left. intros x.
-        apply lprop_left; intros HP.
-        apply lprop_right. now exists x.
-    Qed.
-
-    Lemma lsep_disj_distr {P Q R : L} :
-      ((P ∨ Q) ∗ R) ⊣⊢ ((P ∗ R) ∨ (Q ∗ R)).
-    Proof.
-      split.
-      - apply lwand_sep_adjoint, lor_left;
-          apply lwand_sep_adjoint.
-        + now apply lor_right1.
-        + now apply lor_right2.
-      - apply lor_left; apply lsep_entails; try reflexivity.
-        + now apply lor_right1.
-        + now apply lor_right2.
-    Qed.
-
-    Lemma lsep_exists_comm {A} {P : A -> L} {Q : L} :
-      (∃ x : A, P x) ∗ Q ⊣⊢ (∃ x : A, P x ∗ Q).
-    Proof.
-      split.
-      - apply lwand_sep_adjoint, lex_left; intros x.
-        apply lwand_sep_adjoint, (lex_right x); reflexivity.
-      - apply lex_left; intros x. apply proper_lsep_entails; [|easy].
-        now apply (lex_right x).
-    Qed.
-
-    Lemma land_prop_left {P : Prop} {Q R : L} :
-      (P -> Q ⊢ R) -> (!! P ∧ Q ⊢ R).
-    Proof.
-      rewrite limpl_and_adjoint.
-      - intros H. apply lprop_left. intros HP.
-        apply limpl_and_adjoint.
-        rewrite land_comm, land_true.
-        auto.
-    Qed.
-
-    Lemma lwand_curry {P Q R : L} :
-      ((P ∗ Q) -∗ R) ⊣⊢ (P -∗ (Q -∗ R)).
-    Proof.
-      split.
-      - rewrite <- lwand_sep_adjoint.
-        rewrite <- lwand_sep_adjoint.
-        rewrite <- lsep_assoc.
-        rewrite lwand_sep_adjoint.
-        reflexivity.
-      - rewrite <- lwand_sep_adjoint.
-        rewrite lsep_assoc.
-        rewrite lwand_sep_adjoint.
-        rewrite lwand_sep_adjoint.
-        reflexivity.
-    Qed.
-
-    Lemma lwand_disj_distr {P Q R : L} :
-      ((P ∨ Q) -∗ R) ⊣⊢ ((P -∗ R) ∧ (Q -∗ R)).
-    Proof.
-      split.
-      - apply land_right.
-        + apply proper_lwand_entails. apply lor_right1.
-          reflexivity. reflexivity.
-        + apply proper_lwand_entails. apply lor_right2.
-          reflexivity. reflexivity.
-      - apply lwand_sep_adjoint.
-        rewrite lsep_comm.
-        apply lwand_sep_adjoint.
-        apply lor_left.
-        + apply lwand_sep_adjoint.
-          rewrite lsep_comm.
-          apply lwand_sep_adjoint.
-          now apply land_left1.
-        + apply lwand_sep_adjoint.
-          rewrite lsep_comm.
-          apply lwand_sep_adjoint.
-          now apply land_left2.
-    Qed.
-
-    Lemma lwand_exists_comm {A} {P : A -> L} {Q : L} :
-      ((∃ x : A, P x) -∗ Q) ⊣⊢ (∀ x : A, P x -∗ Q).
-    Proof.
-      split.
-      - apply lall_right. intros x.
-        apply proper_lwand_entails; [|easy].
-        now apply (lex_right x).
-      - apply lwand_sep_adjoint. rewrite lsep_comm.
-        apply lwand_sep_adjoint. apply lex_left. intros x.
-        apply lwand_sep_adjoint. rewrite lsep_comm.
-        apply lwand_sep_adjoint. now apply (lall_left x).
-    Qed.
-
-    Lemma lwand_emp (P : L) :
-      (lemp -∗ P) ⊣⊢ P.
-    Proof.
-      split.
-      - rewrite <- lsep_emp. now apply lwand_sep_adjoint.
-      - apply lwand_sep_adjoint. now rewrite lsep_emp.
-    Qed.
-
-    Lemma lentails_apply {P Q : L} :
-      (⊤ ⊢ P) -> ((P → Q) ⊢ Q).
-    Proof.
-      intros H. transitivity ((P → Q) ∧ P).
-      - apply land_right. easy.
-        transitivity (@lprop L True); auto.
-        apply ltrue_right.
-      - apply limpl_and_adjoint. easy.
-    Qed.
-
-    Lemma lentails_apply' {P Q R : L} :
-      (R ⊢ P) -> ((P → Q) ∧ R ⊢ Q).
-    Proof.
-      intros H. transitivity ((P → Q) ∧ P).
-      apply proper_land_entails; easy.
-      apply limpl_and_adjoint; easy.
-    Qed.
-
-    Lemma limpl_false {P : L} :
-      (⊥ → P) ⊣⊢ ⊤.
-    Proof.
-      split.
-      - apply ltrue_right.
-      - apply limpl_and_adjoint. rewrite land_false.
-        apply lfalse_left.
-    Qed.
-
-    Lemma lall_true {A} :
-      (∀ x : A, ⊤) ⊣⊢@{L} ⊤.
-    Proof.
-      split.
-      - apply ltrue_right.
-      - apply lall_right. intros _. apply ltrue_right.
-    Qed.
-
-    Lemma lprop_intro_impl {P : Prop} (Q R : L) :
-      (P -> Q ⊢ R) ->
-      (Q ⊢ !! P → R).
-    Proof.
-      intros H.
-      apply limpl_and_adjoint.
-      rewrite land_comm.
-      apply limpl_and_adjoint.
-      apply lprop_left. intros HP.
-      apply limpl_and_adjoint.
-      rewrite land_comm, land_true.
-      now apply H.
-    Qed.
-
-    Lemma lprop_intro_wand {P : Prop} (Q R : L) :
-      (P -> Q ⊢ R) ->
-      (Q ⊢ !! P -∗ R).
-    Proof.
-      intros H.
-      apply lwand_sep_adjoint.
-      rewrite lsep_comm.
-      apply lwand_sep_adjoint.
-      apply lprop_left. intros HP.
-      apply lwand_sep_adjoint.
-      rewrite lsep_true.
-      now apply H.
-    Qed.
-
-    Lemma lprop_wand_impl {P : Prop} {Q : L} :
-      (!! P -∗ Q) ⊣⊢ (!! P → Q).
-    Proof.
-      split.
-      - apply lprop_intro_impl. intros HP.
-        rewrite <- (lwand_emp Q) at 2.
-        apply proper_lwand_entails; [|easy].
-        now apply lprop_right.
-      - apply lprop_intro_wand. intros HP.
-        rewrite <- land_true.
-        apply limpl_and_adjoint.
-        apply proper_limpl_entails; [|easy].
-        now apply lprop_right.
-    Qed.
-
-    Lemma lprop_sep_and {P : Prop} {Q : L} :
-      (!! P ∗ Q) ⊣⊢ (!! P ∧ Q).
-    Proof.
-      split.
-      - apply land_right.
-        + apply lwand_sep_adjoint.
-          apply lprop_left; intros Hfml.
-          now apply lwand_sep_adjoint, lprop_right.
-        + rewrite <- (lsep_true Q) at 2.
-          apply proper_lsep_entails; [apply ltrue_right|easy].
-      - apply land_prop_left; intros Hfml. rewrite <- lsep_true at 1.
-        apply proper_lsep_entails; [|easy].
-        now apply lprop_right.
-    Qed.
-
-  End Facts.
-
-End sep.
-Export sep.
+End WithBi.
